% \item \begin{enumerate}
% \item Invalid
% \item Consider the case where $UD = \{a\} $, $F = \{\}$, $H = \{\}$, and $G = % \{a\}$.
% \end{enumerate}

\setcounter{enumi}{1}
\item \begin{enumerate}
\item Valid
\item Consider, for the sake of contradiction, that an interpretation exists where the premises are true and the conclusion is false. Then there exists an element, $ a $, for which $ \lnot (\lnot Ga \lif \lnot Fa) $. This is equivalent to $ \lnot Ga $ and $ Fa $ (this is the only way to falsify the conclusion). Then, $ Fa \lif Ga $ must be false. This contradicts the premise, therefore the conclusion is valid
\item \begin{myproof}
1.& \forall x (Fx \lif Gx) & Premise \\
2.& Fc \lif Gc & UI(1) \\
3.& \lnot Gc \lif \lnot Fc & ContraPos(2) \\
4.& \forall x (\lnot Gx \lif \lnot Fx) & UG(3) \\
\end{myproof}
\end{enumerate}

% \item \begin{enumerate}
% \item Invalid
% \item Consider the case where $UD = \{a\}$, $F = \{\}$, and $G = \{a\}$.
% \end{enumerate}

% \item \begin{enumerate}
% \item Invalid
% \item Consider the case where $UD = \{a\}$, $F = \{a\}$, $G = \{\}$, and $H = % \{a\}$.
% \end{enumerate}

%%% Local Variables: 
%%% mode: latex 
%%% TeX-master: "hw2" 
%%% End: 